state/Compiler.fst
@@ -51,7 +51,7 @@ let src_language1 : language sem_state = {
 noeq
 type tgt_interface1 = {
   ct : fl:_ -> inv : (heap -> Type0) -> prref: mref_pred -> hrel : FStar.Preorder.preorder heap -> Type u#a;
-  c_ct : targetlang default_spec (ct AllOps (Mktuple3?._1 default_spec) (Mktuple3?._2 default_spec) (Mktuple3?._3 default_spec));
+  c_ct : targetlang concrete_spec (ct AllOps (inv_c) (prref_c) (hrel_c));
 }
 
 type ctx_tgt1 (i:tgt_interface1) =
@@ -66,14 +66,14 @@ type ctx_tgt1 (i:tgt_interface1) =
   i.ct fl inv prref hrel
 
 type prog_tgt1 (i:tgt_interface1) =
-  i.ct AllOps (Mktuple3?._1 default_spec) (Mktuple3?._2 default_spec) (Mktuple3?._3 default_spec) ->
+  i.ct AllOps (inv_c) (prref_c) (hrel_c) ->
   SST int (fun _ -> True) (fun _ _ _ -> True)
 
 type whole_tgt1 = (unit -> SST int (fun _ -> True) (fun _ _ _ -> True))
 
-val instantiate_ctx_tgt1 : (#i:tgt_interface1) -> ctx_tgt1 i -> i.ct AllOps (Mktuple3?._1 default_spec) (Mktuple3?._2 default_spec) (Mktuple3?._3 default_spec)
+val instantiate_ctx_tgt1 : (#i:tgt_interface1) -> ctx_tgt1 i -> i.ct AllOps (inv_c) (prref_c) (hrel_c)
 let instantiate_ctx_tgt1 c =
-  c (Mktuple3?._1 default_spec) (Mktuple3?._2 default_spec) (Mktuple3?._3 default_spec) tl_read tl_write tl_alloc
+  c (inv_c) (prref_c) (hrel_c) tl_read tl_write tl_alloc
 
 val link_tgt1 : #i:tgt_interface1 -> prog_tgt1 i -> ctx_tgt1 i -> whole_tgt1
 let link_tgt1 p c =
@@ -159,10 +159,10 @@ type src_interface2 = {
 
 type ctx_src2 (i:src_interface2) =
   i.pt ->
-  SST int (fun h0 -> True) (fun h0 _ h1 -> (Mktuple3?._3 default_spec) h0 h1)
+  SST int (fun h0 -> True) (fun h0 _ h1 -> (hrel_c) h0 h1)
 
 type prog_src2 (i:src_interface2) = i.pt
-type whole_src2 = unit -> SST int (fun h0 -> True) (fun h0 _ h1 -> (Mktuple3?._3 default_spec) h0 h1)
+type whole_src2 = unit -> SST int (fun h0 -> True) (fun h0 _ h1 -> (hrel_c) h0 h1)
 
 let link_src2 (#i:src_interface2) (p:prog_src2 i) (c:ctx_src2 i) : whole_src2 =
   fun () -> c p
@@ -180,7 +180,7 @@ let src_language2 : language sem_state = {
 noeq
 type tgt_interface2 = {
   pt : fl:_ -> inv : (heap -> Type0) -> prref: mref_pred -> hrel : FStar.Preorder.preorder heap -> Type u#a;
-  c_pt : targetlang default_spec (pt AllOps (Mktuple3?._1 default_spec) (Mktuple3?._2 default_spec) (Mktuple3?._3 default_spec));
+  c_pt : targetlang concrete_spec (pt AllOps (inv_c) (prref_c) (hrel_c));
 }
 
 type ctx_tgt2 (i:tgt_interface2) =
@@ -196,14 +196,14 @@ type ctx_tgt2 (i:tgt_interface2) =
   STFlag int fl (fun h0 -> inv h0) (fun h0 _ h1 -> h0 `hrel` h1 /\ inv h1) (** TODO: to check if the program should be an arrow because we don't enforce prref **)
 
 type prog_tgt2 (i:tgt_interface2) =
-  i.pt AllOps (Mktuple3?._1 default_spec) (Mktuple3?._2 default_spec) (Mktuple3?._3 default_spec)
+  i.pt AllOps (inv_c) (prref_c) (hrel_c)
 
-type whole_tgt2 = (unit -> SST int (fun h0 -> True) (fun h0 _ h1 -> (Mktuple3?._3 default_spec) h0 h1))
+type whole_tgt2 = (unit -> SST int (fun h0 -> True) (fun h0 _ h1 -> (hrel_c) h0 h1))
 
 val link_tgt2 : #i:tgt_interface2 -> prog_tgt2 i -> ctx_tgt2 i -> whole_tgt2
 let link_tgt2 p c =
   fun () ->
-    c (Mktuple3?._1 default_spec) (Mktuple3?._2 default_spec) (Mktuple3?._3 default_spec)
+    c (inv_c) (prref_c) (hrel_c)
       tl_read tl_write tl_alloc
       p
 
@@ -224,7 +224,7 @@ let comp_int_src_tgt2 (i:src_interface2) : tgt_interface2 = {
 
 val backtranslate_ctx2 : (#i:src_interface2) -> ctx_tgt2 (comp_int_src_tgt2 i) -> src_language2.ctx i
 let backtranslate_ctx2 #i ct ps =
-  ct #AllOps (Mktuple3?._1 default_spec) (Mktuple3?._2 default_spec) (Mktuple3?._3 default_spec)
+  ct #AllOps (inv_c) (prref_c) (hrel_c)
       tl_read tl_write tl_alloc (i.c_pt.export ps)
 
 val compile_pprog2 : (#i:src_interface2) -> prog_src2 i -> prog_tgt2 (comp_int_src_tgt2 i)
