state/HigherOrderContracts.fst
@@ -15,7 +15,7 @@ instance witnessable_err : witnessable err = {
   satisfy = (fun _ _ -> True);
 }
 
-instance targetlang_err : targetlang default_spec err = {
+instance targetlang_err pspec : targetlang pspec err = {
   wt = witnessable_err
 }
 
@@ -24,29 +24,29 @@ type resexn a = either a err
 class exportable_from (styp: Type u#a) = {
   [@@@no_method] c_styp : witnessable styp;
   [@@@no_method] ityp : Type u#b;
-  [@@@no_method] c_ityp : targetlang default_spec ityp;
+  [@@@no_method] c_ityp : interm ityp;
   [@@@no_method] export : styp -> ityp;
-  [@@@no_method] lemma_export_preserves_prref : x:styp -> Lemma (requires (c_styp.satisfy x (Mktuple3?._2 default_spec))) (ensures (c_ityp.wt.satisfy (export x) (Mktuple3?._2 default_spec)))
+  [@@@no_method] lemma_export_preserves_prref : x:styp -> Lemma (requires (c_styp.satisfy x (prref_c))) (ensures (c_ityp.wt.satisfy (export x) (prref_c)))
 }
 
 class safe_importable_to (styp: Type u#a) = {
   [@@@no_method] c_styp : witnessable styp;
   [@@@no_method] ityp : Type u#b;
-  [@@@no_method] c_ityp : targetlang default_spec ityp;
+  [@@@no_method] c_ityp : interm ityp;
   [@@@no_method] safe_import : ityp -> styp;
-  [@@@no_method] lemma_safe_import_preserves_prref : x:ityp -> Lemma (requires (c_ityp.wt.satisfy x (Mktuple3?._2 default_spec))) (ensures (c_styp.satisfy (safe_import x) (Mktuple3?._2 default_spec)))
+  [@@@no_method] lemma_safe_import_preserves_prref : x:ityp -> Lemma (requires (c_ityp.wt.satisfy x (prref_c))) (ensures (c_styp.satisfy (safe_import x) (prref_c)))
 }
 
 class importable_to (styp: Type u#a) = {
   [@@@no_method] c_styp : witnessable styp;
   [@@@no_method] ityp : Type u#b;
-  [@@@no_method] c_ityp : targetlang default_spec ityp;
+  [@@@no_method] c_ityp : interm ityp;
   [@@@no_method] import : ityp -> resexn styp;
-  [@@@no_method] lemma_import_preserves_prref : x:ityp -> Lemma (requires (c_ityp.wt.satisfy x (Mktuple3?._2 default_spec))) (ensures ((witnessable_sum styp err).satisfy (import x) (Mktuple3?._2 default_spec)))
+  [@@@no_method] lemma_import_preserves_prref : x:ityp -> Lemma (requires (c_ityp.wt.satisfy x (prref_c))) (ensures ((witnessable_sum styp err).satisfy (import x) (prref_c)))
 }
 
 (** Exportable instances **)
-instance targetlang_is_exportable t {| c1:targetlang default_spec t |} : exportable_from t = {
+instance targetlang_is_exportable t {| c1:interm t |} : exportable_from t = {
   c_styp = c1.wt;
   ityp = t;
   c_ityp = solve;
@@ -56,7 +56,7 @@ instance targetlang_is_exportable t {| c1:targetlang default_spec t |} : exporta
 instance exportable_unit : exportable_from unit = {
   c_styp = witnessable_unit;
   ityp = unit;
-  c_ityp = solve;
+  c_ityp = targetlang_unit _;
   export = (fun x -> x);
   lemma_export_preserves_prref = (fun _ -> ())
 }
@@ -64,7 +64,7 @@ instance exportable_unit : exportable_from unit = {
 instance exportable_err : exportable_from err = {
   c_styp = witnessable_err;
   ityp = err;
-  c_ityp = solve;
+  c_ityp = targetlang_err _;
   export = (fun x -> x);
   lemma_export_preserves_prref = (fun _ -> ())
 }
@@ -72,7 +72,7 @@ instance exportable_err : exportable_from err = {
 instance exportable_int : exportable_from int = {
   c_styp = witnessable_int;
   ityp = int;
-  c_ityp = solve;
+  c_ityp = targetlang_int _;
   export = (fun x -> x);
   lemma_export_preserves_prref = (fun _ -> ())
 }
@@ -80,7 +80,7 @@ instance exportable_int : exportable_from int = {
 instance exportable_option t {| c:exportable_from t |} : exportable_from (option t) = {
   c_styp = witnessable_option t #c.c_styp;
   ityp = option c.ityp;
-  c_ityp = targetlang_option default_spec c.ityp #c.c_ityp;
+  c_ityp = targetlang_option _ c.ityp #c.c_ityp;
   export = (fun x -> match x with | Some x -> Some (c.export x) | None -> None);
   lemma_export_preserves_prref = (fun x -> match x with | Some x -> c.lemma_export_preserves_prref x | None -> ())
 }
@@ -88,7 +88,7 @@ instance exportable_option t {| c:exportable_from t |} : exportable_from (option
 instance exportable_sum t1 t2 {| c1:exportable_from t1 |} {| c2:exportable_from t2 |} : exportable_from (either t1 t2) = {
   c_styp = witnessable_sum t1 t2 #c1.c_styp #c2.c_styp;
   ityp = either c1.ityp c2.ityp;
-  c_ityp = targetlang_sum default_spec _ _ #c1.c_ityp #c2.c_ityp;
+  c_ityp = targetlang_sum _ _ _ #c1.c_ityp #c2.c_ityp;
   export = (fun x -> match x with | Inl x -> Inl (c1.export x) | Inr x -> Inr (c2.export x));
   lemma_export_preserves_prref = (fun x ->
     match x with | Inl x -> c1.lemma_export_preserves_prref x | Inr x -> c2.lemma_export_preserves_prref x)
@@ -97,7 +97,7 @@ instance exportable_sum t1 t2 {| c1:exportable_from t1 |} {| c2:exportable_from 
 instance exportable_resexn t {| c:exportable_from t |} : exportable_from (resexn t) = {
   c_styp = witnessable_sum t err #c.c_styp;
   ityp = resexn c.ityp;
-  c_ityp = targetlang_sum default_spec c.ityp err #c.c_ityp;
+  c_ityp = targetlang_sum _ c.ityp err #c.c_ityp;
   export = (fun x -> match x with | Inl x -> Inl (c.export x) | Inr err -> Inr err);
   lemma_export_preserves_prref = (fun x -> match x with | Inl x -> c.lemma_export_preserves_prref x | Inr err -> ())
 }
@@ -105,7 +105,7 @@ instance exportable_resexn t {| c:exportable_from t |} : exportable_from (resexn
 instance exportable_pair t1 t2 {| c1:exportable_from t1 |} {| c2:exportable_from t2 |} : exportable_from (t1 * t2) = {
   c_styp = witnessable_pair t1 t2 #c1.c_styp #c2.c_styp;
   ityp = c1.ityp * c2.ityp;
-  c_ityp = targetlang_pair default_spec _ _ #c1.c_ityp #c2.c_ityp;
+  c_ityp = targetlang_pair _ _ _ #c1.c_ityp #c2.c_ityp;
   export = (fun (x1, x2) -> (c1.export x1, c2.export x2));
   lemma_export_preserves_prref = (fun (x1, x2) -> c1.lemma_export_preserves_prref x1; c2.lemma_export_preserves_prref x2)
 }
@@ -113,7 +113,7 @@ instance exportable_pair t1 t2 {| c1:exportable_from t1 |} {| c2:exportable_from
 instance exportable_ref t {| c:tc_shareable_type t |} : exportable_from (ref t) = {
   c_styp = witnessable_mref t _ #solve;
   ityp = ref t;
-  c_ityp = solve;
+  c_ityp = targetlang_ref _ t #c;
   export = (fun x -> x);
   lemma_export_preserves_prref = (fun _ -> ());
 }
@@ -134,14 +134,14 @@ instance exportable_arrow
   {| c2:exportable_from t2 |}
   (pre:(t1 -> st_pre))
   (post:(x:t1 -> h0:heap -> st_post' (resexn t2) (pre x h0)))
-  (_:squash (forall x h0 r h1. post x h0 r h1 ==> post_targetlang_arrow default_spec #(resexn t2) #(witnessable_sum t2 err #c2.c_styp) h0 r h1))
-  (check:(x:t1 -> ST (either unit err) (pre_targetlang_arrow default_spec #_ #c1.c_styp x) (fun h0 r h1 -> h0==h1 /\ (Inl? r ==> pre x h0))))
+  (_:squash (forall x h0 r h1. post x h0 r h1 ==> post_interm_arrow #(resexn t2) #(witnessable_sum t2 err #c2.c_styp) h0 r h1))
+  (check:(x:t1 -> ST (either unit err) (pre_interm_arrow #_ #c1.c_styp x) (fun h0 r h1 -> h0==h1 /\ (Inl? r ==> pre x h0))))
                              (** ^ the fact that the check has a pre-condition means that the check does not have to enforce it
                                  e.g., the invariant on the heap **)
   : exportable_from (x:t1 -> ST (resexn t2) (pre x) (post x)) = {
   c_styp = witnessable_arrow t1 (resexn t2) pre post;
-  ityp = mk_targetlang_arrow default_spec c1.ityp #c1.c_ityp.wt (resexn c2.ityp) #(witnessable_sum c2.ityp err #c2.c_ityp.wt);
-  c_ityp = targetlang_arrow default_spec c1.ityp (resexn c2.ityp) #_ #(targetlang_sum default_spec c2.ityp err) ;
+  ityp = mk_interm_arrow c1.ityp #c1.c_ityp.wt (resexn c2.ityp) #(witnessable_sum c2.ityp err #c2.c_ityp.wt);
+  c_ityp = targetlang_arrow _ c1.ityp (resexn c2.ityp) #_ #(targetlang_sum _ c2.ityp err) ;
   export = (fun (f:(x:t1 -> ST (resexn t2) (pre x) (post x))) (x:c1.ityp) ->
     match c1.import x with
     | Inl x' -> begin
@@ -160,7 +160,7 @@ instance exportable_arrow
 }
 
 (** Importable instances **)
-instance targetlang_is_safely_importable t {| c1:targetlang default_spec t |} : safe_importable_to t = {
+instance targetlang_is_safely_importable t {| c1:interm t |} : safe_importable_to t = {
   c_styp = c1.wt;
   ityp = t;
   c_ityp = solve;
@@ -179,7 +179,7 @@ instance safe_importable_is_importable t {| c1:safe_importable_to t |} : importa
 instance safe_importable_unit : safe_importable_to unit = {
   c_styp = witnessable_unit;
   ityp = unit;
-  c_ityp = solve;
+  c_ityp = targetlang_unit _;
   safe_import = (fun x -> x);
   lemma_safe_import_preserves_prref = (fun _ -> ())
 }
@@ -187,7 +187,7 @@ instance safe_importable_unit : safe_importable_to unit = {
 instance safe_importable_err : safe_importable_to err = {
   c_styp = witnessable_err;
   ityp = err;
-  c_ityp = solve;
+  c_ityp = targetlang_err _;
   safe_import = (fun x -> x);
   lemma_safe_import_preserves_prref = (fun _ -> ())
 }
@@ -195,7 +195,7 @@ instance safe_importable_err : safe_importable_to err = {
 instance importable_option t {| c:importable_to t |} : importable_to (option t) = {
   c_styp = witnessable_option t #c.c_styp;
   ityp = option c.ityp;
-  c_ityp = targetlang_option default_spec c.ityp #c.c_ityp;
+  c_ityp = targetlang_option _ c.ityp #c.c_ityp;
   import = (fun x ->
     match x with
     | Some x -> begin
@@ -213,7 +213,7 @@ instance importable_option t {| c:importable_to t |} : importable_to (option t) 
 instance importable_sum t1 t2 {| c1:importable_to t1 |} {| c2:importable_to t2 |} : importable_to (either t1 t2) = {
   c_styp = witnessable_sum t1 t2 #c1.c_styp #c2.c_styp;
   ityp = either c1.ityp c2.ityp;
-  c_ityp = targetlang_sum default_spec _ _ #c1.c_ityp #c2.c_ityp;
+  c_ityp = targetlang_sum _ _ _ #c1.c_ityp #c2.c_ityp;
   import = (fun x ->
     match x with
     | Inl x -> begin
@@ -235,7 +235,7 @@ instance importable_sum t1 t2 {| c1:importable_to t1 |} {| c2:importable_to t2 |
 instance safe_importable_ref t {| c:tc_shareable_type t |} : safe_importable_to (ref t) = {
   c_styp = witnessable_mref t _ #solve;
   ityp = ref t;
-  c_ityp = solve;
+  c_ityp = targetlang_ref _ t;
   safe_import = (fun x -> x);
   lemma_safe_import_preserves_prref = (fun _ -> ())
 }
@@ -256,7 +256,7 @@ instance import_refinement t {| c:importable_to t |} (p:t->Type0) (check:(x:t ->
 instance safe_importable_resexn t {| c:importable_to t |} : safe_importable_to (resexn t) = {
   c_styp = witnessable_sum t err #c.c_styp;
   ityp = resexn c.ityp;
-  c_ityp = targetlang_sum default_spec c.ityp err #c.c_ityp;
+  c_ityp = targetlang_sum _ c.ityp err #c.c_ityp;
   safe_import = (fun x ->
     match x with
     | Inl x -> begin
@@ -277,7 +277,7 @@ type cb_capture_check (t1:Type) (t2:Type) {| c2: witnessable t2 |}
   (post:(x:t1 -> h0:heap -> st_post' t2 (pre x h0)))
   (x:t1)
   (eh0:FStar.Ghost.erased heap{pre x eh0}) =
-  (r:t2 -> ST (resexn unit) (fun h1 -> post_targetlang_arrow default_spec eh0 r h1) (fun h1 rck h1' ->
+  (r:t2 -> ST (resexn unit) (fun h1 -> post_interm_arrow eh0 r h1) (fun h1 rck h1' ->
     h1 == h1' /\ (Inl? rck ==> post x eh0 r h1)))
 
 type capture_check
@@ -294,14 +294,14 @@ instance safe_importable_arrow
   {| c2:importable_to t2 |}
   (pre:(t1 -> st_pre))
   (post:(x:t1 -> h0:heap -> st_post' (resexn t2) (pre x h0)))
-  (_:squash (forall (x:t1) h0. pre x h0 ==> pre_targetlang_arrow default_spec #_ #c1.c_styp x h0))
-  (_:squash (forall (x:t1) h0 e h1. pre x h0 /\ post_targetlang_arrow default_spec #_ #(witnessable_sum t2 err #c2.c_styp) h0 (Inr e) h1 ==> post x h0 (Inr e) h1))
+  (_:squash (forall (x:t1) h0. pre x h0 ==> pre_interm_arrow #_ #c1.c_styp x h0))
+  (_:squash (forall (x:t1) h0 e h1. pre x h0 /\ post_interm_arrow #_ #(witnessable_sum t2 err #c2.c_styp) h0 (Inr e) h1 ==> post x h0 (Inr e) h1))
   (capture_check:capture_check t1 (resexn t2) #(witnessable_sum _ err #c2.c_styp) pre post)
   : safe_importable_to (x:t1 -> ST (resexn t2) (pre x) (post x)) = {
   c_styp = witnessable_arrow t1 (resexn t2) pre post;
-  ityp = mk_targetlang_arrow default_spec c1.ityp #c1.c_ityp.wt (resexn c2.ityp) #(witnessable_sum c2.ityp err #c2.c_ityp.wt);
-  c_ityp = targetlang_arrow default_spec c1.ityp (resexn c2.ityp) #_ #(targetlang_sum default_spec c2.ityp err #c2.c_ityp);
-  safe_import = (fun (f:mk_targetlang_arrow default_spec c1.ityp #c1.c_ityp.wt (resexn c2.ityp) #(witnessable_sum c2.ityp err #c2.c_ityp.wt)) (x:t1) ->
+  ityp = mk_interm_arrow c1.ityp #c1.c_ityp.wt (resexn c2.ityp) #(witnessable_sum c2.ityp err #c2.c_ityp.wt);
+  c_ityp = targetlang_arrow _ c1.ityp (resexn c2.ityp) #_ #(targetlang_sum _ c2.ityp err #c2.c_ityp);
+  safe_import = (fun (f:mk_interm_arrow c1.ityp #c1.c_ityp.wt (resexn c2.ityp) #(witnessable_sum c2.ityp err #c2.c_ityp.wt)) (x:t1) ->
     c1.lemma_export_preserves_prref x;
     let (| _, check |) = capture_check x in
     let x' = c1.export x in
@@ -315,12 +315,12 @@ instance safe_importable_arrow
   lemma_safe_import_preserves_prref = (fun _ -> ())
 }
 
-type f_eqx = x:ref int -> SST (resexn unit) (requires (fun h0 -> satisfy x (Mktuple3?._2 default_spec))) (ensures (fun h0 r h1 -> Inr? r \/ sel h0 x == sel h1 x))
+type f_eqx = x:ref int -> SST (resexn unit) (requires (fun h0 -> satisfy x (prref_c))) (ensures (fun h0 r h1 -> Inr? r \/ sel h0 x == sel h1 x))
 
 let f_eqx_is_safe_importable : safe_importable_to f_eqx =
   safe_importable_arrow
     (ref int) unit
-    (fun x -> sst_pre (fun h0 -> satisfy x (Mktuple3?._2 default_spec)))
+    (fun x -> sst_pre (fun h0 -> satisfy x (prref_c)))
     (fun x -> sst_post _ _ (fun h0 r h1 -> Inr? r \/ sel h0 x == sel h1 x))
     ()
     ()
@@ -332,7 +332,7 @@ let f_eqx_is_safe_importable : safe_importable_to f_eqx =
         (fun res -> if x = sst_read rx then Inl () else Inr (Contract_failure "x has changed")) in
       (| eh0, check |))
 
-val unsafe_f : mk_targetlang_arrow default_spec (ref int) (resexn unit)
+val unsafe_f : mk_interm_arrow (ref int) (resexn unit)
 let unsafe_f x =
   recall (contains_pred x);
   recall (is_shared x);
@@ -345,14 +345,14 @@ let safe_f = f_eqx_is_safe_importable.safe_import unsafe_f
 //                                                   ^---^---cannot depend on x
 
 type f_xeq5 = x:ref int -> SST (resexn int)
-  (requires (fun h0 -> sel h0 x == 5 /\ satisfy x (Mktuple3?._2 default_spec)))
-  (ensures (fun h0 r h1 -> (Inr? r \/ (Inl? r /\ Inl?.v r == 2)) /\ ((Mktuple3?._3 default_spec) h0 h1)))
+  (requires (fun h0 -> sel h0 x == 5 /\ satisfy x (prref_c)))
+  (ensures (fun h0 r h1 -> (Inr? r \/ (Inl? r /\ Inl?.v r == 2)) /\ ((hrel_c) h0 h1)))
 
 let f_xeq5_is_exportable : exportable_from f_xeq5 =
   exportable_arrow
     (ref int) int
-    (fun x -> sst_pre (fun h0 -> sel h0 x == 5 /\ satisfy x (Mktuple3?._2 default_spec)))
-    (fun x -> sst_post (resexn int) _ (fun h0 r h1 -> (Inr? r \/ (Inl? r /\ Inl?.v r == 2)) /\ ((Mktuple3?._3 default_spec) h0 h1)))
+    (fun x -> sst_pre (fun h0 -> sel h0 x == 5 /\ satisfy x (prref_c)))
+    (fun x -> sst_post (resexn int) _ (fun h0 r h1 -> (Inr? r \/ (Inl? r /\ Inl?.v r == 2)) /\ ((hrel_c) h0 h1)))
     ()
     (fun x ->
       recall (contains_pred x);
